Complexitylib/Circuits/Unrolling/Defs.lean
@@ -3,7 +3,7 @@ Copyright (c) 2026 Samuel Schlesinger. All rights reserved.
 Released under Apache 2.0 license as described in the file LICENSE.
 Authors: Samuel Schlesinger
 -/
-import Complexitylib.Circuits.Encoding.Formula.Defs
+import Complexitylib.Circuits.Encoding.Fragment.Defs
 import Complexitylib.Models.TuringMachine
 import Mathlib.Data.Fintype.Sum
 import Mathlib.Logic.Equiv.Fin.Basic
